Ajustement CompCert

src/fresh/CompCert/cfrontend/MoSel.v
@@ -1,207 +1,81 @@
-From iris.proofmode Require Export base intro_patterns spec_patterns
-     sel_patterns coq_tactics reduction
-     coq_tactics ltac_tactics.
 Require Import FunctionalExtensionality.
-From iris Require Import bi.bi proofmode.tactics proofmode.monpred proofmode.reduction.
+Require Import Errors.
 Require Import SepSet.
-
-Global Set Warnings "-convert_concl_no_check".
-
-Module SepBasicCore.
-
-  Ltac inversion_star h P :=
-    match goal with
-    | H : (_ \* _) _ |- _ =>
-      let W := fresh h in
-      let w := fresh P in
-      inversion H as (W&w);
-      let W := fresh h in
-      destruct w as (W&w);
-      do 3 (let w0 := fresh P in
-            destruct w as (w0&w))
-    end.
-
-  Local Ltac Fresh :=
-    let x := iFresh in
-    match x with
-    | IAnon ?x =>
-      let x := eval compute in (ascii_of_pos (x + 64)) in
-          let x := eval compute in (append "H" (string_of_list_ascii [x])) in
-              let env := iGetCtx in
-              let P := reduction.pm_eval (envs_lookup x env) in
-              match P with
-              | None => x
-              | Some _ => Fresh
-              end
-    | _ => fail "iFresh returns " x " sometimes."
-    end.
-
-  (*h should be in the environment *)
-  Local Ltac norm h :=
-    let env := iGetCtx in
-    let P := reduction.pm_eval (envs_lookup h env) in
-    match P with
-    | None => fail "assert false"
-    | Some (false, ?P) =>
-      match P with
-      | bi_exist ?Q => let x := fresh "x" in (iDestruct h as (x) h; norm h)
-      | bi_sep ?Q ?W =>
-        let x := Fresh in
-        let y := Fresh in
-        eapply tac_and_destruct with h _ x y _ _ _;
-        [ pm_reflexivity | pm_reduce; iSolveTC | pm_reduce; norm x; norm y]
-      | bi_pure (and ?P ?Q) =>
-        let x := Fresh in
-        eapply tac_and_destruct with h _ h x _ _ _;
-        [pm_reflexivity
-        |pm_reduce; iSolveTC
-        |pm_reduce; norm h; norm x]
-      | bi_pure _ => iPure h as ?
-      | bi_wand _ _ => iDestruct (h with "[]") as h; [progress auto | norm h]
-      | bi_absorbingly _ =>
-        let name := Fresh in
-        let name_mod := eval compute in (append ">" name) in
-            iPoseProof h as name; iDestruct name as name_mod; norm name
-      | _ =>
-        match h with
-        | IAnon _ =>
-          let x := Fresh in
-          iPoseProof h as x
-        | _ => idtac
-        end
-      end
-    | Some (true,?P) => idtac
-    end.
-
-  (* (List.fold norm) in Ltac *)
-  Local Ltac norm_list l :=
-    match l with
-    | [] => idtac
-    | ?h :: ?t => norm h ; norm_list t
-    end.
-
-
-  Ltac norm_all :=
-    iStartProof;
-    let env := iGetCtx in
-    let list_ident := eval compute in (rev (envs_dom env)) in
-        norm_list list_ident; auto.
-
-  Tactic Notation "iNorm" := norm_all.
-
-End SepBasicCore.
-
 Require Import Ctypes.
 
-Module gensym.
-  Import Errors.
-  Export SepBasicCore.
-  Export SepSet.
+Definition ident := positive.
 
-  Definition ident := positive.
+Record generator : Type := mkgenerator { gen_next : ident;
+                                         gen_trail: list (ident * type)
+                             }.
 
-  Record generator : Type := mkgenerator { gen_next : ident;
-                                           gen_trail: list (ident * type)
-                                         }.
+Parameter first_unused_ident : unit -> ident.
 
-  Parameter first_unused_ident : unit -> ident.
-
-  Definition initial_generator (x : unit) : generator :=
-    mkgenerator (first_unused_ident x) nil.
+Definition initial_generator (x : unit) : generator :=
+  mkgenerator (first_unused_ident x) nil.
 
 
-  Inductive mon (X : Type) : Type :=
-  | ret : X -> mon X
-  | errorOp : Errors.errmsg -> mon X
-  | gensymOp : type -> (ident -> mon X) -> mon X
-  | trailOp : unit -> (list (ident * type) -> mon X) -> mon X.
+Inductive mon (X : Type) : Type :=
+| ret : X -> mon X
+| errorOp : Errors.errmsg -> mon X
+| gensymOp : type -> (ident -> mon X) -> mon X
+| trailOp : unit -> (list (ident * type) -> mon X) -> mon X.
 
-  Arguments errorOp [X].
-  Arguments gensymOp [X].
-  Arguments trailOp [X].
-  Arguments ret {_} x.
+Arguments errorOp [X].
+Arguments gensymOp [X].
+Arguments trailOp [X].
+Arguments ret {_} x.
 
 
-  Fixpoint bind {X Y} (m : mon X) (f : X -> mon Y) : mon Y :=
-    match m with
-    | ret x => f x
-    | errorOp e => errorOp e
-    | gensymOp t g => gensymOp t (fun x => bind (g x) f)
-    | trailOp _ g => trailOp tt (fun x => bind (g x) f)
-    end.
-
-  Notation "'let!' x ':=' e1 'in' e2" := (bind e1 (fun x => e2)) (x name, at level 90).
-
-  Notation "'ret!' v" := (ret v) (v name, at level 90).
-
-  Definition error {X} (e : Errors.errmsg) : mon X := errorOp e.
-  Definition gensym (t : type) : mon ident := gensymOp t ret.
-  Definition trail (_ : unit): mon (list (ident * type)) := trailOp tt ret.
-
-  Lemma lid : forall X Y (a : X) (f : X -> mon Y), bind (ret a) f = f a.
-  Proof. auto. Qed.
-
-  Lemma rid : forall X (m : mon X), bind m ret = m.
-  Proof.
-    fix m 2.
-    destruct m0.
-    1 - 2 : reflexivity.
-    all : simpl; do 2 f_equal.
-    2 : destruct u; auto.
-    all : apply functional_extensionality; intro; apply m.
-  Qed.
-
-  Lemma ass_bind : forall X Y Z (m : mon X) f (g : Y -> mon Z),
-      bind (bind m f) g = bind m (fun x => bind (f x) g).
-  Proof.
-    fix m 4.
-    destruct m0; intros.
-    1 - 2 : reflexivity.
-    all : simpl; do 2 f_equal; apply functional_extensionality; intro; apply m.
-  Qed.
-
-  Fixpoint eval {X} (m : mon X) : generator -> res (generator * X) :=
+Fixpoint bind {X Y} (m : mon X) (f : X -> mon Y) : mon Y :=
   match m with
-  | ret v => fun s => OK (s, v)
-  | errorOp e => fun s => Error e
-  | gensymOp ty f =>
-    fun s =>
-      let h := gen_trail s in
-      let n := gen_next s in
-      eval (f n) (mkgenerator (Pos.succ n) ((n,ty) :: h))
-  | trailOp _ f =>
-    fun s =>
-      let h := gen_trail s in
-      eval (f h) s
+  | ret x => f x
+  | errorOp e => errorOp e
+  | gensymOp t g => gensymOp t (fun x => bind (g x) f)
+  | trailOp _ g => trailOp tt (fun x => bind (g x) f)
   end.
 
-Definition run {X} (m: mon X): res X :=
-  match eval m (initial_generator tt) with
-  | OK (_, v) => OK v
-  | Error e => Error e
+Notation "'let!' x ':=' e1 'in' e2" := (bind e1 (fun x => e2)) (x name, at level 90).
+
+Notation "'ret!' v" := (ret v) (v name, at level 90).
+
+Definition error {X} (e : Errors.errmsg) : mon X := errorOp e.
+Definition gensym (t : type) : mon ident := gensymOp t ret.
+Definition trail (_ : unit): mon (list (ident * type)) := trailOp tt ret.
+
+Lemma lid : forall X Y (a : X) (f : X -> mon Y), bind (ret a) f = f a.
+Proof. auto. Qed.
+
+Lemma rid : forall X (m : mon X), bind m ret = m.
+Proof.
+  fix m 2.
+  destruct m0.
+  1 - 2 : reflexivity.
+  all : simpl; do 2 f_equal.
+  2 : destruct u; auto.
+  all : apply functional_extensionality; intro; apply m.
+Qed.
+
+Lemma ass_bind : forall X Y Z (m : mon X) f (g : Y -> mon Z),
+    bind (bind m f) g = bind m (fun x => bind (f x) g).
+Proof.
+  fix m 4.
+  destruct m0; intros.
+  1 - 2 : reflexivity.
+  all : simpl; do 2 f_equal; apply functional_extensionality; intro; apply m.
+Qed.
+
+Fixpoint wp {X} (e1 : mon X) (Q : X -> iProp) : iProp :=
+  match e1 with
+  | ret v => Q v
+  | errorOp e => True
+  | gensymOp _ f => ∀ l, & l -∗ wp (f l) Q
+  | trailOp _ f => ∀ l, wp (f l) Q
   end.
 
-End gensym.
-
-Module weakestpre_gensym.
-  Export gensym.
-  Export proofmode.monpred.
-  Export SepBasicCore.
-  Import reduction.
-
-  (* Definition iProp := monPred biInd (@hpropI ident positive_eq_dec pos_countable). *)
-
-  Fixpoint wp {X} (e1 : mon X) (Q : X -> iProp) : iProp :=
-    match e1 with
-    | ret v => Q v
-    | errorOp e => True
-    | gensymOp _ f => ∀ l, & l -∗ wp (f l) Q
-    | trailOp _ f => ∀ l, wp (f l) Q
-    end.
-
-  Notation "'{{' P } } e {{ v ; Q } }" := (P -∗ wp e (fun v => Q))
-                                            (at level 20,
-                                             format "'[hv' {{  P  } }  '/  ' e  '/'  {{  v ;  Q  } } ']'").
+Notation "'{{' P } } e {{ v ; Q } }" := (P ⊢ wp e (fun v => Q))
+                                          (at level 20,
+                                            format "'[hv' {{  P  } }  '/  ' e  '/'  {{  v ;  Q  } } ']'").
 
 (** triple rules *)
 
@@ -228,13 +102,13 @@ Proof.
 Qed.
 
 Lemma ret_spec {X} (v : X) H (Q : X -> iProp) :
-  (H ⊢ Q v) -> ⊢{{ H }} ret v {{ v'; Q v' }}.
+  (H ⊢ Q v) -> {{ H }} ret v {{ v'; Q v' }}.
 Proof. simpl; iIntros. iApply H0; auto. Qed.
 
 Lemma bind_spec {X Y} (e : mon X) (f : X -> mon Y) Q Q' H :
-   (⊢{{ H }} e {{ v; Q' v }}) ->
-    (∀ v, ⊢{{ Q' v }} (f v) {{ v'; Q v' }}) ->
-    ⊢ {{ H }} (bind e f) {{ v; Q v}}.
+  ({{ H }} e {{ v; Q' v }}) ->
+  (∀ v, {{ Q' v }} (f v) {{ v'; Q v' }}) ->
+  {{ H }} (bind e f) {{ v; Q v}}.
 Proof.
   intros. iIntros "HA".
   iApply (wp_bind e f _ Q' with "[HA]").
@@ -243,10 +117,10 @@ Proof.
 Qed.
 
 Lemma consequence {X} H H' (Q : X -> iProp) (Q' : X -> iProp) (e : mon X) :
-  (⊢{{ H' }} e {{ v; Q' v }}) ->
+  ({{ H' }} e {{ v; Q' v }}) ->
   (forall v, Q' v ⊢ Q v) ->
   (H ⊢ H') ->
-  ⊢{{ H }} e {{ v; Q v }}.
+  {{ H }} e {{ v; Q v }}.
 Proof.
   intros. iIntros "HA". iDestruct (H2 with "HA") as "HA".
   iDestruct (H0 with "HA") as "HA". iApply (wp_consequence with "HA"). iIntros "*". iApply H1.
@@ -257,142 +131,159 @@ Lemma frame_bind : forall (P : iProp), ⊢ P -∗ emp ∗ P.
 Proof. iIntros "* $". Qed.
 
 Lemma frame {X} H R Q (e : mon X) :
-  (⊢{{ H }} e {{ v; Q v }}) ->
-  ⊢{{ H ∗ R }} e {{ v; Q v ∗ R }}.
+  ({{ H }} e {{ v; Q v }}) ->
+  {{ H ∗ R }} e {{ v; Q v ∗ R }}.
 Proof.
   intro P. iIntros "[HA HC]". iApply (wp_consequence with "[HA]").
   iApply P; auto. iIntros; iFrame.
 Qed.
 
 Lemma intro_true_r {X} H Q (e : mon X) :
-  (⊢{{ emp ∗ H }} e {{ v; Q v }}) ->
-  ⊢{{ H }} e {{ v; Q v }}.
+  ({{ emp ∗ H }} e {{ v; Q v }}) ->
+  {{ H }} e {{ v; Q v }}.
 Proof.
   intro P. iIntros "HA". iApply (P with "[HA]").
   iFrame.
 Qed.
 
 Lemma exists_spec {X Y} v' H (Q : X -> Y -> iProp) (e : mon X) :
-  (⊢{{ H }} e {{ v; Q v v' }}) ->
-  ⊢{{ H }} e {{ v; ∃ t, Q v t }}.
+  ({{ H }} e {{ v; Q v v' }}) ->
+  {{ H }} e {{ v; ∃ t, Q v t }}.
 Proof.
-  intros. iIntros "HA". iApply consequence; eauto.
+  intros. iApply consequence. iApply H0.  all : eauto.
 Qed.
 
 Ltac Frame := eapply intro_true_r; eapply frame.
 
 (** Effects rules *)
 
-Lemma rule_gensym t : ⊢{{ emp }} gensym t {{ l; & l }}.
+Lemma rule_gensym t : {{ emp }} gensym t {{ l; & l }}.
 Proof. simpl; auto. Qed.
 
-Lemma rule_error {X} P (Q : X -> iProp) e : ⊢{{ P }} error e {{ v; Q v }}.
+Lemma rule_error {X} P (Q : X -> iProp) e : {{ P }} error e {{ v; Q v }}.
 Proof. auto. Qed.
 
-Lemma rule_trail  : ⊢{{ emp }} trail tt {{ _; emp  }}.
+Lemma rule_trail  : {{ emp }} trail tt {{ _; emp  }}.
 Proof. auto. Qed.
 
-End weakestpre_gensym.
 
-Module adequacy.
-  Import Errors.
-  Export weakestpre_gensym.
 
-  Definition inject_aux n :=
-    List.map Pos.of_nat
-             (seq (Pos.to_nat (first_unused_ident ()))
-                  (Pos.to_nat n - Pos.to_nat (first_unused_ident ()))).
+Definition inject_aux n :=
+  List.map Pos.of_nat
+    (seq (Pos.to_nat (first_unused_ident ()))
+       (Pos.to_nat n - Pos.to_nat (first_unused_ident ()))).
 
-  Lemma inject_last : forall n,
-      Pos.le (first_unused_ident ()) n -> inject_aux (Pos.succ n) = inject_aux n ++ [n].
-  Proof.
-    intros n lt. unfold inject_aux. rewrite <- (Pos2Nat.id n).
-    assert (forall (n : nat), [Pos.of_nat n] = Pos.of_nat n :: map Pos.of_nat nil) by auto.
-    rewrite H. rewrite <- map_cons. rewrite <- map_app. f_equal.
-    rewrite Pos2Nat.id. assert (forall (n : nat), [n] = seq n 1) by auto. rewrite H0.
-    assert ((Pos.to_nat (first_unused_ident ())) +
+Lemma inject_last : forall n,
+    Pos.le (first_unused_ident ()) n -> inject_aux (Pos.succ n) = inject_aux n ++ [n].
+Proof.
+  intros n lt. unfold inject_aux. rewrite <- (Pos2Nat.id n).
+  assert (forall (n : nat), [Pos.of_nat n] = Pos.of_nat n :: map Pos.of_nat nil) by auto.
+  rewrite H. rewrite <- map_cons. rewrite <- map_app. f_equal.
+  rewrite Pos2Nat.id. assert (forall (n : nat), [n] = seq n 1) by auto. rewrite H0.
+  assert ((Pos.to_nat (first_unused_ident ())) +
             (Pos.to_nat n - Pos.to_nat (first_unused_ident ()))
-            = Pos.to_nat n) by lia.
-    rewrite <- H1 at 2. rewrite <- seq_app. f_equal. lia.
-  Qed.
+          = Pos.to_nat n) by lia.
+  rewrite <- H1 at 2. rewrite <- seq_app. f_equal. lia.
+Qed.
 
-  Lemma next_disjoint : forall n, Pos.le (first_unused_ident ()) n ->  (inject_aux n) ## [n].
+Lemma next_disjoint : forall n, Pos.le (first_unused_ident ()) n ->  (inject_aux n) ## [n].
+Proof.
+  repeat intro. inversion H1. subst.
+  - unfold inject_aux in H0. apply elem_of_list_In in H0. apply Coqlib.list_in_map_inv in H0.
+    destruct H0 as [x [P0 P2]].
+    apply in_seq in P2. destruct P2. lia.
+  - inversion H4.
+Qed.
+
+Lemma unused_nil : inject_aux (first_unused_ident ()) = nil.
+Proof.
+  unfold inject_aux. rewrite PeanoNat.Nat.sub_diag. simpl. reflexivity.
+Qed.
+
+Definition inject n : (@gset MoSel.ident positive_eq_dec pos_countable) :=
+  list_to_set (inject_aux n).
+
+Lemma unused_map : inject (first_unused_ident ()) = ∅.
+Proof.
+  unfold inject. rewrite unused_nil. simpl. auto.
+Qed.
+
+Lemma inject_last_set : forall n,
+    Pos.le (first_unused_ident ()) n -> inject (Pos.succ n) = {[ n ]} ∪ (inject n).
+Proof.
+  intros. unfold inject. rewrite inject_last; auto.
+  rewrite list_to_set_app_L. simpl. rewrite union_empty_r_L.
+  rewrite union_comm_L. auto.
+Qed.
+
+Lemma inject_disjoint : forall n, Pos.le (first_unused_ident ()) n -> inject n ## {[ n ]}.
+Proof.
+  intros. apply disjoint_singleton_r. unfold inject.
+  apply not_elem_of_list_to_set. intro. eapply next_disjoint; eauto.
+  constructor.
+Qed.
+
+Fixpoint eval {X} (m : mon X) : generator -> res (generator * X) :=
+  match m with
+  | ret v => fun s => OK (s, v)
+  | errorOp e => fun s => Error e
+  | gensymOp ty f =>
+      fun s =>
+        let h := gen_trail s in
+        let n := gen_next s in
+        eval (f n) (mkgenerator (Pos.succ n) ((n,ty) :: h))
+  | trailOp _ f =>
+      fun s =>
+        let h := gen_trail s in
+        eval (f h) s
+  end.
+
+Definition run {X} (m: mon X): res X :=
+  match eval m (initial_generator tt) with
+  | OK (_, v) => OK v
+  | Error e => Error e
+  end.
+
+
+Section Eval_Adequacy.
+  Variable X: Type.
+  Implicit Type m: mon X.
+  Implicit Type P: iProp.
+  Implicit Type Q: X -> iProp.
+  Implicit Type v: X.
+
+  Lemma adequacy_wp : forall m Q g_init g_res v,
+      Pos.le (first_unused_ident tt) (gen_next g_init) ->
+      (&& (inject (gen_next g_init)) ⊢ wp m Q) ->
+      eval m g_init = Errors.OK (g_res, v) ->
+      (Q v) () (inject (gen_next g_res)).
   Proof.
-    repeat intro. inversion H1. subst.
-    - unfold inject_aux in H0. apply elem_of_list_In in H0. apply Coqlib.list_in_map_inv in H0.
-      destruct H0 as [x [P0 P2]].
-      apply in_seq in P2. destruct P2. lia.
-    - inversion H4.
+    fix ind 1.
+    destruct m; intros.
+    - inversion H1; subst. apply soundness. iApply H0.
+    - inversion H1.
+    - simpl in *. eapply ind.
+      3 : apply H1.
+      + simpl. lia.
+      + iIntros "HA". simpl. rewrite inject_last_set; auto.
+        iDestruct (heap_ctx_split_sing with "HA") as "[HA HB]".
+        apply inject_disjoint; auto. iDestruct (H0 with "HA") as "HA".
+        iApply ("HA" with "HB").
+    - simpl in *. eapply ind; eauto. iIntros "HA". iApply (H0 with "HA").
   Qed.
 
-  Lemma unused_nil : inject_aux (first_unused_ident ()) = nil.
+  Lemma adequacy_init : forall e Q g v,
+      (⊢ wp e Q) ->
+      eval e (initial_generator tt) = Errors.OK (g, v) ->
+      (Q v) () (inject (gen_next g)).
   Proof.
-    unfold inject_aux. rewrite PeanoNat.Nat.sub_diag. simpl. reflexivity.
+    intros. eapply adequacy_wp; eauto. simpl. lia.
+    rewrite unused_map. auto.
   Qed.
-
-  Definition inject n : (@gset ident positive_eq_dec pos_countable) :=
-    list_to_set (inject_aux n).
-
-  Lemma unused_map : inject (first_unused_ident ()) = ∅.
-  Proof.
-    unfold inject. rewrite unused_nil. simpl. auto.
-  Qed.
-
-  Lemma inject_last_set : forall n,
-      Pos.le (first_unused_ident ()) n -> inject (Pos.succ n) = {[ n ]} ∪ (inject n).
-  Proof.
-    intros. unfold inject. rewrite inject_last; auto.
-    rewrite list_to_set_app_L. simpl. rewrite union_empty_r_L.
-    rewrite union_comm_L. auto.
-  Qed.
-
-  Lemma inject_disjoint : forall n, Pos.le (first_unused_ident ()) n -> inject n ## {[ n ]}.
-  Proof.
-    intros. apply disjoint_singleton_r. unfold inject.
-    apply not_elem_of_list_to_set. intro. eapply next_disjoint; eauto.
-    constructor.
-  Qed.
-
-
-  Section Eval_Adequacy.
-    Variable X: Type.
-    Implicit Type m: mon X.
-    Implicit Type P: iProp.
-    Implicit Type Q: X -> iProp.
-    Implicit Type v: X.
-
-    Lemma adequacy_wp : forall m Q g_init g_res v,
-        Pos.le (first_unused_ident tt) (gen_next g_init) ->
-        (&& (inject (gen_next g_init)) ⊢ wp m Q) ->
-        eval m g_init = Errors.OK (g_res, v) ->
-        (Q v) () (inject (gen_next g_res)).
-    Proof.
-      fix ind 1.
-      destruct m; intros.
-      - inversion H1; subst. apply soundness. iApply H0.
-      - inversion H1.
-      - simpl in *. eapply ind.
-        3 : apply H1.
-        + simpl. lia.
-        + iIntros "HA". simpl. rewrite inject_last_set; auto.
-          iDestruct (heap_ctx_split_sing with "HA") as "[HA HB]".
-          apply inject_disjoint; auto. iDestruct (H0 with "HA") as "HA".
-          iApply ("HA" with "HB").
-      - simpl in *. eapply ind; eauto. iIntros "HA". iApply (H0 with "HA").
-    Qed.
-
-    Lemma adequacy_init : forall e Q g v,
-        (⊢ wp e Q) ->
-        eval e (initial_generator tt) = Errors.OK (g, v) ->
-        (Q v) () (inject (gen_next g)).
-    Proof.
-      intros. eapply adequacy_wp; eauto. simpl. lia.
-      rewrite unused_map. auto.
-    Qed.
 
   Lemma adequacy_core : forall e Q g_init v g_res H,
       Pos.le (first_unused_ident tt) (gen_next g_init) ->
-      (&& (inject (gen_next g_init)) ⊢ H) -> (⊢ {{ H }} e {{ v; Q v }}) ->
+      (&& (inject (gen_next g_init)) ⊢ H) -> ({{ H }} e {{ v; Q v }}) ->
       eval e g_init = Errors.OK (g_res, v) ->
       (Q v) () (inject (gen_next g_res)).
   Proof.
@@ -401,36 +292,36 @@ Module adequacy.
   Qed.
 
   Lemma adequacy_triple_init : forall e Q v g H,
-      (⊢ H) -> (⊢ {{ H }} e {{ v; Q v }}) ->
+      (⊢ H) -> ({{ H }} e {{ v; Q v }}) ->
       eval e (initial_generator tt) = Errors.OK (g, v) ->
       (Q v) () (inject (gen_next g)).
   Proof.
     intros. eapply adequacy_init; eauto. iApply H1; eauto.
   Qed.
 
-  End Eval_Adequacy.
+End Eval_Adequacy.
 
-  Lemma adequacy_wp_pure {X} : forall (e : mon X) (Q : X -> Prop) g_init v g_res,
-      Pos.le (first_unused_ident tt) (gen_next g_init) ->
-      (&& (inject (gen_next g_init)) ⊢ wp e (fun v =>  ⌜Q v⌝)) ->
-      eval e g_init = Errors.OK (g_res, v) ->
-      Q v.
-  Proof.
-    intros. apply (soundness_pure (inject (gen_next g_res))). iApply completeness.
-    eapply (adequacy_wp _ _ _ _ _ _ H H0 H1).
-  Qed.
+Lemma adequacy_wp_pure {X} : forall (e : mon X) (Q : X -> Prop) g_init v g_res,
+    Pos.le (first_unused_ident tt) (gen_next g_init) ->
+    (&& (inject (gen_next g_init)) ⊢ wp e (fun v =>  ⌜Q v⌝)) ->
+    eval e g_init = Errors.OK (g_res, v) ->
+    Q v.
+Proof.
+  intros. apply (soundness_pure (inject (gen_next g_res))). iApply completeness.
+  eapply (adequacy_wp _ _ _ _ _ _ H H0 H1).
+Qed.
 
-  Lemma adequacy_pure {X} : forall (e : mon X) (Q : X -> Prop) g_init v g_res H,
-      Pos.le (first_unused_ident tt) (gen_next g_init) ->
-      (&& (inject (gen_next g_init)) ⊢ H) -> (⊢ {{ H }} e {{ v; ⌜ Q v ⌝}}) ->
-      eval e g_init = Errors.OK (g_res, v) ->
-      Q v.
-  Proof.
-    intros. eapply adequacy_wp_pure; eauto. iIntros "HA". iDestruct (H1 with "HA") as "HA".
-    iDestruct (H2 with "HA") as "$".
-  Qed.
+Lemma adequacy_pure {X} : forall (e : mon X) (Q : X -> Prop) g_init v g_res H,
+    Pos.le (first_unused_ident tt) (gen_next g_init) ->
+    (&& (inject (gen_next g_init)) ⊢ H) -> ({{ H }} e {{ v; ⌜ Q v ⌝}}) ->
+    eval e g_init = Errors.OK (g_res, v) ->
+    Q v.
+Proof.
+  intros. eapply adequacy_wp_pure; eauto. iIntros "HA". iDestruct (H1 with "HA") as "HA".
+  iDestruct (H2 with "HA") as "$".
+Qed.
 
-  Section Adequacy.
+Section Adequacy.
   Variable X: Type.
   Implicit Type m: mon X.
   Implicit Type P: iProp.
@@ -438,7 +329,7 @@ Module adequacy.
   Implicit Type v: X.
 
   Lemma adequacy: forall m Q v,
-      (⊢ {{ emp }} m {{ v; ⌜ Q v ⌝}}) ->
+      ({{ emp }} m {{ v; ⌜ Q v ⌝}}) ->
       run m = OK v -> Q v.
   Proof.
     intros m.
@@ -452,6 +343,4 @@ Module adequacy.
     inversion H0.
   Qed.
 
-  End Adequacy.
-
-End adequacy.
+End Adequacy.
